wip: delta beta

DeltaBetaReduction.v
@@ -2,22 +2,233 @@ Require Import PeanoNat.
 
 Require Export SystemFR.RedTactics.
 Require Export SystemFR.ScalaDepSugar.
+Require Export SystemFR.EquivalentContext.
 
 Opaque reducible_values.
 
-Inductive delta_beta_reduction: context -> tree -> tree -> Prop :=
-| DBTrue: forall Γ, delta_beta_reduction Γ ttrue ttrue
-| DBFalse: forall Γ, delta_beta_reduction Γ tfalse tfalse
+Reserved Notation "'[' Γ ⊨ t1 '⤳*' t2 ']'" (Γ at level 60, t1 at level 60).
+
+Inductive cbv_open_value: tree -> Prop :=
+| OVVar: forall x, cbv_open_value (fvar x term_var)
+| OVUnit: cbv_open_value uu
+| OVZero: cbv_open_value zero
+| OVSucc: forall v, cbv_open_value v -> cbv_open_value (succ v)
+| OVFalse: cbv_open_value tfalse
+| OVTrue: cbv_open_value ttrue
+| OVPair: forall v1 v2, cbv_open_value v1 -> cbv_open_value v2 -> cbv_open_value (pp v1 v2)
+| OVLambda: forall t, cbv_open_value (notype_lambda t)
+| OVLeft : forall v, cbv_open_value v -> cbv_open_value (tleft v)
+| OVRight: forall v, cbv_open_value v -> cbv_open_value (tright v)
 .
 
-(*Notation "'[' Γ ⊨ t1 '⤳' t2 ']'" := (delta_beta_step Γ t1 t2)
-  (Γ at level 60, t1 at level 60). *)
-Notation "'[' Γ ⊨ t1 '⤳*' t2 ']'" := (delta_beta_reduction Γ t1 t2)
-  (Γ at level 60, t1 at level 60).
+Hint Constructors cbv_open_value: open_values.
+
+Inductive delta_beta_reduction: context -> tree -> tree -> Prop :=
+| DBVar:
+    forall Γ x ty t v,
+      wf t 0 ->
+      lookup Nat.eq_dec Γ x = Some (T_singleton ty t) ->
+      [ Γ ⊨ t ⤳* v ] ->
+      [ Γ ⊨ fvar x term_var ⤳* v ]
+
+| DBPair:
+    forall Γ t1 t2 v1 v2,
+      [ Γ ⊨ t1 ⤳* v1 ] ->
+      [ Γ ⊨ t2 ⤳* v2 ] ->
+      [ Γ ⊨ pp t1 t2 ⤳* pp v1 v2 ]
+
+| DBFirst:
+    forall Γ t v1 v2,
+      is_erased_term v1 ->
+      is_erased_term v2 ->
+      wf v1 0 ->
+      wf v2 0 ->
+      subset (fv v1) (support Γ) ->
+      subset (fv v2) (support Γ) ->
+      cbv_open_value v1 ->
+      cbv_open_value v2 ->
+      [ Γ ⊨ t ⤳* pp v1 v2 ] ->
+      [ Γ ⊨ pi1 t ⤳* v1 ]
+
+| DBSecond:
+    forall Γ t v1 v2,
+      is_erased_term v1 ->
+      is_erased_term v2 ->
+      wf v1 0 ->
+      wf v2 0 ->
+      subset (fv v1) (support Γ) ->
+      subset (fv v2) (support Γ) ->
+      cbv_open_value v1 ->
+      cbv_open_value v2 ->
+      [ Γ ⊨ t ⤳* pp v1 v2 ] ->
+      [ Γ ⊨ pi2 t ⤳* v2 ]
+
+| DBRefl:
+    forall Γ v,
+      is_erased_term v ->
+      wf v 0 ->
+      subset (fv v) (support Γ) ->
+      cbv_open_value v ->
+      [ Γ ⊨ v ⤳* v ] (* when evaluation is finished *)
+
+where "'[' Γ ⊨ t1 '⤳*' t2 ']'" := (delta_beta_reduction Γ t1 t2).
+
+Lemma delta_beta_var:
+  forall Θ Γ x ty t v,
+    wf t 0 ->
+    lookup Nat.eq_dec Γ x = Some (T_singleton ty t) ->
+    [ Θ; Γ ⊨ t ≡ v ] ->
+    [ Θ; Γ ⊨ fvar x term_var ≡ v ].
+Proof.
+  unfold open_equivalent, T_singleton;
+    repeat step || t_lookup || erewrite satisfies_same_support in * by eauto.
+  unshelve epose proof (satisfies_lookup2 _ _ _ _ _ _ H3 H0 matched);
+    repeat step || simp_red || open_none || rewrite shift_nothing2 in * by eauto with wf;
+    eauto using equivalent_trans.
+Qed.
+
+Lemma delta_beta_pair:
+  forall Θ Γ t1 t2 t1' t2',
+    [ Θ; Γ ⊨ t1 ≡ t1' ] ->
+    [ Θ; Γ ⊨ t2 ≡ t2' ] ->
+    [ Θ; Γ ⊨ pp t1 t2 ≡ pp t1' t2' ].
+Proof.
+  unfold open_equivalent; repeat step || apply equivalent_pp; eauto.
+Qed.
+
+Lemma open_equivalent_refl:
+  forall Θ Γ t,
+    is_erased_term t ->
+    wf t 0 ->
+    subset (fv t) (support Γ) ->
+    [ Θ; Γ ⊨ t ≡ t ].
+Proof.
+  unfold open_equivalent; intros; apply equivalent_refl; steps;
+    eauto with erased fv wf.
+Qed.
+
+Lemma equivalent_pi1_pp:
+  forall v1 v2,
+    is_erased_term v1 ->
+    is_erased_term v2 ->
+    wf v1 0 ->
+    wf v2 0 ->
+    pfv v1 term_var = nil ->
+    pfv v2 term_var = nil ->
+    cbv_value v1 ->
+    cbv_value v2 ->
+    [ pi1 (pp v1 v2) ≡ v1 ].
+Proof.
+  intros; equivalent_star.
+Qed.
+
+Lemma equivalent_pi2_pp:
+  forall v1 v2,
+    is_erased_term v1 ->
+    is_erased_term v2 ->
+    wf v1 0 ->
+    wf v2 0 ->
+    pfv v1 term_var = nil ->
+    pfv v2 term_var = nil ->
+    cbv_value v1 ->
+    cbv_value v2 ->
+    [ pi2 (pp v1 v2) ≡ v2 ].
+Proof.
+  intros; equivalent_star.
+Qed.
+
+Lemma lookup_value:
+  forall l x v,
+    are_values l ->
+    lookup Nat.eq_dec l x = Some v ->
+    cbv_value v.
+Proof.
+  induction l; steps; eauto.
+Qed.
+
+Lemma close_open_value:
+  forall v l,
+    cbv_open_value v ->
+    are_values l ->
+    subset (fv v) (support l) ->
+    cbv_value (substitute v l).
+Proof.
+  induction 1; repeat step || sets;
+    eauto using lookup_value;
+    try solve [ unfold subset in *; repeat step || t_lookup; eauto with exfalso ];
+    eauto with values.
+Qed.
+
+Lemma satisfies_are_values:
+  forall l ρ Γ,
+    valid_interpretation ρ ->
+    satisfies (reducible_values ρ) Γ l ->
+    are_values l.
+Proof.
+  induction l; repeat step || step_inversion satisfies; eauto with values.
+Qed.
+
+Lemma close_open_value2:
+  forall v Γ ρ l,
+    cbv_open_value v ->
+    valid_interpretation ρ ->
+    satisfies (reducible_values ρ) Γ l ->
+    subset (fv v) (support Γ) ->
+    cbv_value (psubstitute v l term_var).
+Proof.
+  intros; eapply close_open_value;
+    repeat step || erewrite satisfies_same_support in * by eauto;
+    eauto with values;
+    eauto using satisfies_are_values.
+Qed.
+
+Lemma delta_beta_first:
+  forall Θ Γ t v1 v2,
+    is_erased_term v1 ->
+    is_erased_term v2 ->
+    wf v1 0 ->
+    wf v2 0 ->
+    subset (fv v1) (support Γ) ->
+    subset (fv v2) (support Γ) ->
+    cbv_open_value v1 ->
+    cbv_open_value v2 ->
+    [ Θ; Γ ⊨ t ≡ pp v1 v2 ] ->
+    [ Θ; Γ ⊨ pi1 t ≡ v1 ].
+Proof.
+  unfold open_equivalent; repeat step || apply equivalent_pp; eauto.
+  eapply equivalent_trans; eauto using equivalent_pi1.
+  apply equivalent_pi1_pp; steps; eauto with erased wf fv;
+    eauto using close_open_value2.
+Qed.
+
+Lemma delta_beta_second:
+  forall Θ Γ t v1 v2,
+    is_erased_term v1 ->
+    is_erased_term v2 ->
+    wf v1 0 ->
+    wf v2 0 ->
+    subset (fv v1) (support Γ) ->
+    subset (fv v2) (support Γ) ->
+    cbv_open_value v1 ->
+    cbv_open_value v2 ->
+    [ Θ; Γ ⊨ t ≡ pp v1 v2 ] ->
+    [ Θ; Γ ⊨ pi2 t ≡ v2 ].
+Proof.
+  unfold open_equivalent; repeat step || apply equivalent_pp; eauto.
+  eapply equivalent_trans; eauto using equivalent_pi2.
+  apply equivalent_pi2_pp; steps; eauto with erased wf fv;
+    eauto using close_open_value2.
+Qed.
 
 Lemma delta_beta_obs_equiv:
   forall Θ Γ t1 t2,
     [ Γ ⊨ t1 ⤳* t2 ] ->
     [ Θ; Γ ⊨ t1 ≡ t2 ].
 Proof.
-Admitted.
+  induction 1; repeat step;
+    eauto using delta_beta_var;
+    eauto using delta_beta_pair;
+    eauto using delta_beta_first;
+    eauto using delta_beta_second;
+    eauto using open_equivalent_refl.
+Qed.
